

## IT5002 Computer Systems and Applications

### Tutorial 1

#### Number Systems

#### SUGGESTED SOLUTIONS

1. In 2's complement representation, "sign extension" is used when we want to represent an  $n$ -bit signed integer as an  $m$ -bit signed integer, where  $m > n$ . We do this by copying the MSB (most significant bit) of the  $n$ -bit number  $m - n$  times to the left of the  $n$ -bit number to create the  $m$ -bit number.

For example, we want to sign-extend 0b0110 to an 8-bit number. Here  $n = 4$ ,  $m = 8$ , and thus we copy the MSB bit 0 four ( $8 - 4$ ) times, giving 0b00000110.

Similarly, if we want to sign-extend 0b1010 to an 8-bit number, we would get 0b1111010.

Show that IN GENERAL, sign extension is value-preserving. For example, 0b00000110 = 0b0110 and 0b1111010 = 0b1010.

*Answer:*

Let  $X$  be the  $n$ -bit signed integer and  $Y$  be the  $m$ -bit signed integer which is the sign-extended version of  $X$ .

If the MSB of  $X$  is zero, this is straightforward, since padding more 0's to the left adds nothing to the final value. If the MSB of  $X$  is one, then it is trickier to prove. In the original  $n$ -bit representation, the MSB has a weight of  $-2^{n-1}$  giving us

$$X = -2^{n-1} + b_{n-2} \cdot 2^{n-2} + b_{n-3} \cdot 2^{n-3} + \dots + b_0.$$

Let  $Z = b_{n-2} \cdot 2^{n-2} + b_{n-3} \cdot 2^{n-3} + \dots + b_0$ , then  $X = -2^{n-1} + Z$ .

In the new  $m$ -bit representation  $Y$  where  $m > n$ , the MSB of  $Y$  has a weight of  $-2^{m-1}$ , and since we copy the MSB (i.e. the leftmost bit) of  $X$  a total of  $m - n$  times, we get

$$Y = -2^{m-1} + 2^{m-2} + 2^{m-3} + \dots + 2^n + 2^{n-1} + Z.$$

For  $Y = X$ , it suffices to show that  $-2^{m-1} + 2^{m-2} + 2^{m-3} + \dots + 2^n + 2^{n-1} = -2^{n-1}$ .

Recall that the sum of a Geometric Progression with  $N$  terms, initial value  $a$  and ratio  $r$  is given by:  $\frac{a(r^N - 1)}{r - 1}$ . We will use this formula to calculate  $2^{m-2} + 2^{m-3} + \dots + 2^n + 2^{n-1}$ , which has  $N = (m - 2) - (n - 1) + 1 = m - n$ ;  $a = 2^{m-2}$  and  $r = 2$ .

$$\begin{aligned} & -2^{m-1} + (2^{m-2} + 2^{m-3} + \dots + 2^n + 2^{n-1}) \\ &= -2^{m-1} + \frac{a(r^N - 1)}{r - 1} \\ &= -2^{m-1} + 2^{n-1}(2^{m-n} - 1) \\ &= -2^{m-1} + 2^{m-1} - 2^{n-1} \\ &= -2^{n-1} \end{aligned}$$

Therefore,  $Y = X$ .

2. We generalize  $(r - 1)$ 's-complement (also called *radix diminished complement*) to include fraction as follows:

$$(r - 1)'s \text{ complement of } N = r^n - r^{-m} - N$$

where  $n$  is the number of integer digits and  $m$  the number of fractional digits. (If there are no fractional digits, then  $m = 0$  and the formula becomes  $r^n - 1 - N$  as given in class.)

For example, the 1's complement of 011.01 is  $(2^3 - 2^{-2}) - 011.01 = (1000 - 0.01) - 011.01 = 111.11 - 011.01 = 100.10$ . (Since 011.01 represents the decimal value 3.25 in 1's complement, this means that -3.25 is represented as 100.10 in 1's complement.)

Perform the following binary subtractions of values represented in 1's complement representation by using addition instead. (Note: Recall that when dealing with complement representations, the two operands must have the same number of digits.)

- (a) 0101.11 - 010.0101  
(b) 010111.101 - 0111010.11

Is sign extension used in your working? If so, highlight it.

Check your answers by converting the operands and answers to their actual decimal values.

**Answers:**

(a) 0101.1100 - 0010.0101 → 0101.1100 + 1101.1010 → **0011.0111<sub>1s</sub>**  
(Check:  $5.75 - 2.3125 = 3.4375$ )

(b) 0010111.101 - 0111010.110 → 0010111.101 + 1000101.001 →  
**1011100.110<sub>1s</sub> = -0100011.001<sub>2</sub>**  
(Check:  $23.625 - 58.75 = -35.125$ )

Note that sign-extension is used above.

Note that two trailing zeroes are added. (This is not sign extension.)

3. Convert the following numbers to fixed-point binary in 2's complement, with 4 bits for the integer portion and 3 bits for the fraction portion.

- (a) 1.75      (b) -2.5      (c) 3.876      (d) 2.1

Using the binary representations you have derived, convert them back into decimal. Comment on the compromise between range and accuracy of the fixed-point binary system.

**Answers:**

(a) 1.75  
(0001.110)<sub>2s</sub>

(b) -2.5  
Begin with 2.5: (0010.100)<sub>2s</sub>. Invert and add 0.001: (1101.100)<sub>2s</sub>

(c) 3.876  
 $0.876 \times 2 = 1.752$   
 $0.752 \times 2 = 1.504$   
 $0.504 \times 2 = 1.008$   
 $0.008 \times 2 = 0.016$  (why perform 4 steps instead of 3?)  
So  $0.876_{10} = 0.1110_{2s} = 0.111_{2s}$   
Answer: (0011.111)<sub>2s</sub>

(d) 2.1

$$0.1 \times 2 = 0.2$$

$$0.2 \times 2 = 0.4$$

$$0.4 \times 2 = 0.8$$

$$0.8 \times 2 = 1.6 \text{ (why perform 4 steps instead of 3?)}$$

$$\text{So } 0.1_{10} = 0.0001_{25} = 0.001_{25}$$

$$\text{Putting it together we have: } 2.1_{10} = (0010.001)_{25}$$

The first two will convert back exactly to 1.75 and -2.5, so that's ok.

For (c), the fraction part is  $0.111_2 = 0.5 + 0.25 + 0.125 = 0.875$ , which is just off the target of 0.876 by 0.001. Not bad.

For (d), the fraction part is  $0.001_2 = 0.125$ . This is off the actual value of 0.1 by 0.025, quite a lot.

Comment: Not all values can be represented exactly, and the precision depends on the number of bits in the fraction part. In this case 3 bits is too little to even represent 0.1, because the smallest fraction it can represent is 0.125.

4. [AY2010/2011 Semester 2 Term Test #1]

How would you represent the decimal value  $-0.078125$  in the IEEE 754 single-precision representation? Express your answer in hexadecimal. Show your working.

**Answer: B D A 0 0 0 0 0**

$$-0.078125 = -0.000101_2 = -1.01 \times 2^{-4}$$

$$\text{Exponent} = -4 + 127 = 123 = 01111011_2$$

$$1 \ 01111011 \ 0100000...$$

$$1011 \ 1101 \ 1010 \ 0000 \ ...$$

$$\text{B D A 0 0 0 0 0}$$

5. Write the following in MIPS Assembly, using as few instructions as possible. You may rewrite the equations if necessary to minimize instructions.

In all parts you can assume that integer variables **a**, **b**, **c** and **d** are mapped to registers \$s0, \$s1, \$s2 and \$s3 respectively. Each part is independent of the others.

a.  $c = a + b$

$\text{add } \$s2, \$s0, \$s1$

b.  $d = a + b - c$

$\text{add } \$s3, \$s0, \$s1 \quad \# d = a + b$

$\text{sub } \$s3, \$s3, \$s2 \quad \# d = (a + b) - c$

c.  $c = 2b + (a - 2)$

$\text{add } \$s2, \$s1, \$s1 \quad \# c = 2b \text{ (alternatively, can do a shift left 1 bit)}$

$\text{addi } \$t0, \$s0, -2 \quad \# \$t0 = a - 2$

add \$s2, \$s2, \$t0 #  $c = 2b + (a - 2)$

d.  $d = 6a + 3(b - 2c)$

Note to TAs: Students may find better solutions than this. Check to ensure that they achieve the equation above.

Rewrite:

$d = 6a + 3b - 6c$

Factorize out 3

$d = 3(2a + b - 2c)$

$= 3(2a - 2c + b)$

$= 3(2(a - c) + b)$

sub \$t0, \$s0, \$s2 #  $t0 = a - c$

sll \$t0, \$t0, 1 #  $t0 = 2(a - c)$

add \$t0, \$t0, \$s1 #  $t0 = 2(a - c) + b$

sll \$t1, \$t0, 2 #  $t1 = 4(2(a - c) + b)$

sub \$s3, \$t1, \$t0 #  $d = 3(2(a - c) + b)$